Tsum5_HK.thy
@@ -16,13 +16,13 @@ primrec tsh :: "nat \<Rightarrow> nat \<Rightarrow> nat event stream \<Rightarro
                         else(if shd ts= \<surd> then (\<up>\<surd> \<bullet> (tsh n p (srt\<cdot>ts)))
                                 else (\<up>(Msg (p + (\<M>\<inverse> (shd ts))))) \<bullet> (tsh n (p +(\<M>\<inverse> (shd ts))) (srt\<cdot> ts))))"
 
-(*Helper for tsum5 like sum5_helper for sum5 but over nat event streams*)
-definition tsum5_helper :: " nat \<Rightarrow> nat event stream \<rightarrow> nat event stream" where
-"tsum5_helper p \<equiv> \<Lambda> ts. (\<Squnion>i. tsh i p ts)"
+(*Helper for tsum5 like sum5_h for sum5 but over nat event streams*)
+definition tsum5_h :: " nat \<Rightarrow> nat event stream \<rightarrow> nat event stream" where
+"tsum5_h p \<equiv> \<Lambda> ts. (\<Squnion>i. tsh i p ts)"
 
 (*Definition of sum5 over timed streams*)
 definition tsum5:: "nat tstream \<rightarrow> nat tstream" where
-"tsum5 \<equiv> (\<Lambda> ts. Abs_tstream (tsum5_helper 0\<cdot>(Rep_tstream ts)))"
+"tsum5 \<equiv> (\<Lambda> ts. Abs_tstream (tsum5_h 0\<cdot>(Rep_tstream ts)))"
 
 
 
@@ -51,7 +51,7 @@ lemma tswellinftick: "ts_well ((\<up>\<surd>)\<infinity>)"
 by (simp add: ts_well_def)
 
 (*Implies that tsh of (\<up>\<surd>)\<infinity> equals (\<up>\<surd>)\<infinity>*)
-lemma tssum5_helpersinf: "tsh (Suc n) p (sinftimes(\<up>\<surd>)) = (\<up>\<surd>) \<bullet> tsh n p (sinftimes (\<up>\<surd>))"
+lemma tsum5_hsinf: "tsh (Suc n) p (sinftimes(\<up>\<surd>)) = (\<up>\<surd>) \<bullet> tsh n p (sinftimes (\<up>\<surd>))"
 by auto
 
 (*tsh i works at most with the first i elements of the input*)
@@ -108,12 +108,12 @@ proof -
 qed
 
 (*#(tsh n p s) = min(n, #s)*)
-lemma cont_lub_tsum5_helper2:
+lemma cont_lub_tsum5_h2:
   "\<forall>s p. stake n\<cdot> (tsh n p s) = tsh n p s "
 by(induct_tac n,auto)
 
-(* tsum5_helper is a continuous function *)
-lemma cont_lub_tsum5_helper: "cont (\<lambda> s. \<Squnion>i. tsh i p s)" 
+(* tsum5_h is a continuous function *)
+lemma cont_lub_tsum5_h: "cont (\<lambda> s. \<Squnion>i. tsh i p s)" 
 apply (rule cont2cont_lub)
 apply (rule ch2ch_fun)
 apply (rule chainI)
@@ -127,10 +127,10 @@ apply (rule allI)
 apply (rule_tac x="i" in exI)
 by (simp add: contlub_tsh)
 
-(*Describes the unfolding of tsum5_helper if the first element of the stream is a natural message*)
-lemma tsum5_helper_scons:"a\<noteq>\<surd> \<Longrightarrow> tsum5_helper n \<cdot>(\<up>a\<bullet>s) = (\<up>(\<M>(n+(\<M>\<inverse> a)))) \<bullet> (tsum5_helper (n+ (\<M>\<inverse> a))\<cdot>s)"  
-apply (simp add: tsum5_helper_def)
-apply (subst beta_cfun, rule cont_lub_tsum5_helper)+
+(*Describes the unfolding of tsum5_h if the first element of the stream is a natural message*)
+lemma tsum5_h_scons:"a\<noteq>\<surd> \<Longrightarrow> tsum5_h n \<cdot>(\<up>a\<bullet>s) = (\<up>(\<M>(n+(\<M>\<inverse> a)))) \<bullet> (tsum5_h (n+ (\<M>\<inverse> a))\<cdot>s)"  
+apply (simp add: tsum5_h_def)
+apply (subst beta_cfun, rule cont_lub_tsum5_h)+
 apply (subst contlub_cfun_arg)
 apply (rule ch2ch_fun, rule ch2ch_fun)
 apply (rule chainI)
@@ -143,10 +143,10 @@ apply (rule fun_belowD [of _ _ "a"])
 apply (smt chain_tsh fun_belowI po_class.chain_def)
 by (simp add: chain_tsh_helper)
 
-(*Describes the unfolding of tsum5_helper if the first element of the stream is a \<surd>*)
-lemma tsum5_helper_scons_tick:"tsum5_helper n \<cdot>(\<up>\<surd>\<bullet>s) = \<up>\<surd> \<bullet> (tsum5_helper n \<cdot>s)"
-apply (simp add: tsum5_helper_def)
-apply (subst beta_cfun, rule cont_lub_tsum5_helper)+
+(*Describes the unfolding of tsum5_h if the first element of the stream is a \<surd>*)
+lemma tsum5_h_scons_tick:"tsum5_h n \<cdot>(\<up>\<surd>\<bullet>s) = \<up>\<surd> \<bullet> (tsum5_h n \<cdot>s)"
+apply (simp add: tsum5_h_def)
+apply (subst beta_cfun, rule cont_lub_tsum5_h)+
 apply (subst contlub_cfun_arg)
 apply (rule ch2ch_fun, rule ch2ch_fun)
 apply (rule chainI)
@@ -159,67 +159,67 @@ apply (rule fun_belowD [of _ _ "n"])
 apply (smt chain_tsh fun_belowI po_class.chain_def)
 by (simp add: chain_tsh_helper)
 
-(*Other lemma with the same meaning as tsum5_helper_scons_tick*)
-lemma tsum5_helper_scons_tick_2: "s=\<up>\<surd>\<bullet>as \<Longrightarrow> tsum5_helper n\<cdot>s = (\<up>\<surd>)\<bullet>(tsum5_helper n\<cdot> as)"
-by (simp add: tsum5_helper_scons_tick)
+(*Other lemma with the same meaning as tsum5_h_scons_tick*)
+lemma tsum5_h_scons_tick_2: "s=\<up>\<surd>\<bullet>as \<Longrightarrow> tsum5_h n\<cdot>s = (\<up>\<surd>)\<bullet>(tsum5_h n\<cdot> as)"
+by (simp add: tsum5_h_scons_tick)
 
-(*Other lemma with the same meaning as tsum5_helper_scons*)
-lemma tsum5_helper_scons_2:"shd s\<noteq>\<surd> \<and> s\<noteq>\<epsilon>\<Longrightarrow> tsum5_helper n \<cdot>s = (\<up>(\<M>(n+(\<M>\<inverse> shd s)))) \<bullet> (tsum5_helper (n+ (\<M>\<inverse> shd s))\<cdot>(srt\<cdot>s))"
-using tsum5_helper_scons
+(*Other lemma with the same meaning as tsum5_h_scons*)
+lemma tsum5_h_scons_2:"shd s\<noteq>\<surd> \<and> s\<noteq>\<epsilon>\<Longrightarrow> tsum5_h n \<cdot>s = (\<up>(\<M>(n+(\<M>\<inverse> shd s)))) \<bullet> (tsum5_h (n+ (\<M>\<inverse> shd s))\<cdot>(srt\<cdot>s))"
+using tsum5_h_scons
 by (metis surj_scons)
 
-lemma tsum5_helper_scons_tick_alternative:"a=\<surd> \<Longrightarrow> tsum5_helper n \<cdot>(\<up>a\<bullet>s) = \<up>a \<bullet> (tsum5_helper n \<cdot>s)"
-by(simp add: tsum5_helper_scons_tick)
+lemma tsum5_h_scons_tick_alternative:"a=\<surd> \<Longrightarrow> tsum5_h n \<cdot>(\<up>a\<bullet>s) = \<up>a \<bullet> (tsum5_h n \<cdot>s)"
+by(simp add: tsum5_h_scons_tick)
 
-(*tsum5_helper of an empty stream is an empty stream*)
-lemma tsum5_empty[simp]: "tsum5_helper p\<cdot>\<epsilon> = \<epsilon>"
-by (simp add: cont_lub_tsum5_helper tsh_bot tsum5_helper_def)
+(*tsum5_h of an empty stream is an empty stream*)
+lemma tsum5_empty[simp]: "tsum5_h p\<cdot>\<epsilon> = \<epsilon>"
+by (simp add: cont_lub_tsum5_h tsh_bot tsum5_h_def)
 
-(*unfolding tsum5_helper with the definition*)
-lemma tsum5_helper_unfold_tsh: "tsum5_helper n \<cdot>input = (\<Squnion>i. tsh i n input)"
-apply (simp add:tsum5_helper_def)
-by (simp add: cont_lub_tsum5_helper)
+(*unfolding tsum5_h with the definition*)
+lemma tsum5_h_unfold_tsh: "tsum5_h n \<cdot>input = (\<Squnion>i. tsh i n input)"
+apply (simp add:tsum5_h_def)
+by (simp add: cont_lub_tsum5_h)
 
 (*Shows that the message of a natural number of an nat event plus 0 is the nat event*)
 lemma msg_plus0[simp]:fixes a::"nat event" shows" a\<noteq>\<surd> \<Longrightarrow>\<M> (0+(\<M>\<inverse> a)) = a"
 by (metis add.left_neutral event.exhaust event.simps(4))
 
-(*shd of tsum5_helper if the head is not \<surd>*)
-lemma tsum5_helper_shd [simp]: "a\<noteq>\<surd> \<Longrightarrow> shd (tsum5_helper n \<cdot>(\<up>a \<bullet> as)) = \<M> (n+(\<M>\<inverse> a))"
-by (simp add: tsum5_helper_scons)
+(*shd of tsum5_h if the head is not \<surd>*)
+lemma tsum5_h_shd [simp]: "a\<noteq>\<surd> \<Longrightarrow> shd (tsum5_h n \<cdot>(\<up>a \<bullet> as)) = \<M> (n+(\<M>\<inverse> a))"
+by (simp add: tsum5_h_scons)
 
-(*shd of tsum5_helper if the head is not \<surd>*)
-lemma tsum5_helper_shd_2 [simp]: "shd s\<noteq>\<surd> \<and> s\<noteq>\<epsilon> \<Longrightarrow> shd (tsum5_helper n \<cdot>s) = \<M> (n+(\<M>\<inverse> shd s))"
-by (simp add: tsum5_helper_scons_2)
+(*shd of tsum5_h if the head is not \<surd>*)
+lemma tsum5_h_shd_2 [simp]: "shd s\<noteq>\<surd> \<and> s\<noteq>\<epsilon> \<Longrightarrow> shd (tsum5_h n \<cdot>s) = \<M> (n+(\<M>\<inverse> shd s))"
+by (simp add: tsum5_h_scons_2)
 
-(*The head of tsum5_helper is the head of the input*)
-lemma tsum5_shd: "shd (tsum5_helper 0\<cdot>ts) = shd ts"
+(*The head of tsum5_h is the head of the input*)
+lemma tsum5_shd: "shd (tsum5_h 0\<cdot>ts) = shd ts"
 apply(cases "ts= \<epsilon>")
 apply simp
 apply(cases "shd ts= \<surd>")
-apply (metis shd1 surj_scons tsum5_helper_scons_tick)
-by (metis msg_plus0 surj_scons tsum5_helper_shd)
+apply (metis shd1 surj_scons tsum5_h_scons_tick)
+by (metis msg_plus0 surj_scons tsum5_h_shd)
 
 (*A stream filtered by \<surd>s only contains \<surd>*)
 lemma "#({\<surd>} \<ominus> s) = Fin (Suc n) \<Longrightarrow> ({\<surd>} \<ominus> s)= (\<up>\<surd>)\<bullet>(srt\<cdot>({\<surd>} \<ominus> s))"
 by (metis Fin_02bot inject_Fin lnzero_def nat.simps(3) sfilter_resl2 singletonD slen_empty_eq surj_scons)
 
-(*#(tsum5_helper s)is at least the length of s*)
-lemma tsum5_helper_slen2: "#s \<le> #(tsum5_helper a\<cdot>s)"
+(*#(tsum5_h s)is at least the length of s*)
+lemma tsum5_h_slen2: "#s \<le> #(tsum5_h a\<cdot>s)"
 apply (rule spec [where x = a])
 apply (rule ind [of _ s], auto)
 apply(subst lnle_def, simp del: lnle_conv)
-by (smt lnsuc_lnle_emb slen_scons tsum5_helper_scons tsum5_helper_scons_tick)
+by (smt lnsuc_lnle_emb slen_scons tsum5_h_scons tsum5_h_scons_tick)
 
-(*The rest of tsum5_helper s is tsum5_helper (srt s) if the head of s is a \<surd>*)
-lemma tsum5_helper_srt_tick: "shd s=\<surd> \<Longrightarrow>srt\<cdot>(tsum5_helper n \<cdot>s) = tsum5_helper n\<cdot> (srt\<cdot>s)"
-by (metis (no_types, lifting) inject_scons lshd_updis stream.sel_rews(2) stream.sel_rews(3) surj_scons tsum5_empty tsum5_helper_scons_tick)
+(*The rest of tsum5_h s is tsum5_h (srt s) if the head of s is a \<surd>*)
+lemma tsum5_h_srt_tick: "shd s=\<surd> \<Longrightarrow>srt\<cdot>(tsum5_h n \<cdot>s) = tsum5_h n\<cdot> (srt\<cdot>s)"
+by (metis (no_types, lifting) inject_scons lshd_updis stream.sel_rews(2) stream.sel_rews(3) surj_scons tsum5_empty tsum5_h_scons_tick)
 
-(*Unfolding the rest of tsum5_helper if the head is not a \<surd>*)
-lemma tsum5_helper_srt: "shd s\<noteq>\<surd> \<Longrightarrow>srt\<cdot>(tsum5_helper n \<cdot>s) = tsum5_helper (n+(\<M>\<inverse> shd s))\<cdot> (srt\<cdot>s)"
+(*Unfolding the rest of tsum5_h if the head is not a \<surd>*)
+lemma tsum5_h_srt: "shd s\<noteq>\<surd> \<Longrightarrow>srt\<cdot>(tsum5_h n \<cdot>s) = tsum5_h (n+(\<M>\<inverse> shd s))\<cdot> (srt\<cdot>s)"
 apply(cases "s=\<epsilon>")
 apply simp
-using tsum5_helper_scons
+using tsum5_h_scons
 proof -
   assume a1: "s \<noteq> \<epsilon>"
   assume a2: "shd s \<noteq> \<surd>"
@@ -228,75 +228,75 @@ proof -
   have "\<And>e s. updis (e::nat event) \<noteq> \<bottom> \<or> (\<epsilon>::nat event stream) = s"
     by simp
   then show ?thesis
-    using f3 a2 a1 by (metis lscons_conv stream.sel_rews(5) tsum5_helper_scons)
+    using f3 a2 a1 by (metis lscons_conv stream.sel_rews(5) tsum5_h_scons)
 qed
 
-(*tsum5_helper has the length of the input*)
-lemma tsum5_helper_slen[simp]: "#(tsum5_helper n\<cdot>s) = #s"
+(*tsum5_h has the length of the input*)
+lemma tsum5_h_slen[simp]: "#(tsum5_h n\<cdot>s) = #s"
 apply (rule spec [where x = n])
 apply (rule ind [of _ s], auto)
-using tsum5_helper_scons
-by (metis slen_scons tsum5_helper_scons_tick)
+using tsum5_h_scons
+by (metis slen_scons tsum5_h_scons_tick)
 
-(*Unfolds tsum5_helper with a \<up>(Msg m) as the input*)
-lemma [simp]: "a\<noteq>\<surd> \<Longrightarrow> tsum5_helper n\<cdot>(\<up>a) = (\<up>(\<M>(n+(\<M>\<inverse> a))))"
-by (metis lscons_conv sup'_def tsum5_empty tsum5_helper_scons)
+(*Unfolds tsum5_h with a \<up>(Msg m) as the input*)
+lemma [simp]: "a\<noteq>\<surd> \<Longrightarrow> tsum5_h n\<cdot>(\<up>a) = (\<up>(\<M>(n+(\<M>\<inverse> a))))"
+by (metis lscons_conv sup'_def tsum5_empty tsum5_h_scons)
 
-(*tsum5_helper of a ts_well \<up>a is \<up>a*)
-lemma tsum5_helper_one[simp]: "ts_well (\<up>a) \<Longrightarrow> tsum5_helper n\<cdot>(\<up>a) = \<up>(a)"
+(*tsum5_h of a ts_well \<up>a is \<up>a*)
+lemma tsum5_h_one[simp]: "ts_well (\<up>a) \<Longrightarrow> tsum5_h n\<cdot>(\<up>a) = \<up>(a)"
 apply(cases "a\<noteq>\<surd>")
 apply (simp add: tsOneTick)
 apply auto
-apply(insert tsum5_helper_scons_tick [of n \<epsilon>])
+apply(insert tsum5_h_scons_tick [of n \<epsilon>])
 by simp
 
 (*Length of tsAbs ts of a timedstream ts*)
 lemma tsAbs_len[simp]: "ts_well s \<Longrightarrow> #(tsAbs\<cdot>(Abs_tstream s)) = #({e. e\<noteq>\<surd>}\<ominus> s)"
 by(subst tsabs_insert, simp)
 
-(*Length of tsum5_helper of a event stream without ticks is eqaul to the length of sum5 of tsAbs*)
-lemma tsum5_helper_sfilter_len: "ts_well s \<Longrightarrow> #(tsum5_helper n\<cdot>({e. e\<noteq>\<surd>}\<ominus>s)) = #(sum5\<cdot>(tsAbs\<cdot>(Abs_tstream s)))"
+(*Length of tsum5_h of a event stream without ticks is eqaul to the length of sum5 of tsAbs*)
+lemma tsum5_h_sfilter_len: "ts_well s \<Longrightarrow> #(tsum5_h n\<cdot>({e. e\<noteq>\<surd>}\<ominus>s)) = #(sum5\<cdot>(tsAbs\<cdot>(Abs_tstream s)))"
 by simp
 
-(*sum5_helper unfolding when the head of the stream is 0 is the parameter concatenated to sum5_helper with the rest of the stream*)
-lemma tsum5_unfold_tsum5: "tsum5_helper n\<cdot>(\<up>(\<M> 0) \<bullet> s) =\<up>(\<M> (0+n)) \<bullet> tsum5_helper n \<cdot>(s)"
-apply(subst tsum5_helper_scons)
+(*sum5_h unfolding when the head of the stream is 0 is the parameter concatenated to sum5_h with the rest of the stream*)
+lemma tsum5_unfold_tsum5: "tsum5_h n\<cdot>(\<up>(\<M> 0) \<bullet> s) =\<up>(\<M> (0+n)) \<bullet> tsum5_h n \<cdot>(s)"
+apply(subst tsum5_h_scons)
 apply simp
 by simp
 
-(*the (Suc nth) element of sum5_helper when the head of the stream is 0 is the nth element of sum5_helper with the rest stream*)
-lemma test2_tsum5_helper_help: "Fin n < #s \<longrightarrow> snth (Suc n) (tsum5_helper m \<cdot>(\<up>(\<M> 0) \<bullet>s)) = snth n (tsum5_helper m \<cdot>s)"
+(*the (Suc nth) element of sum5_h when the head of the stream is 0 is the nth element of sum5_h with the rest stream*)
+lemma test2_tsum5_h_help: "Fin n < #s \<longrightarrow> snth (Suc n) (tsum5_h m \<cdot>(\<up>(\<M> 0) \<bullet>s)) = snth n (tsum5_h m \<cdot>s)"
 apply(induction n)
 apply(subst tsum5_unfold_tsum5)
 apply simp
 by (simp add: tsum5_unfold_tsum5)
 
-(*the (Suc nth) element of tsum5_helper when the head of the stream is \<surd> is the nth element of tsum5_helper with the rest stream*)
-lemma tsum5_suc_snth_tick:"Fin n < #s \<and> shd s =\<surd> \<Longrightarrow> snth (Suc n) (tsum5_helper m\<cdot>s) = snth n (tsum5_helper m\<cdot>(srt\<cdot>s))"
-apply(subst tsum5_helper_scons_tick_2)
+(*the (Suc nth) element of tsum5_h when the head of the stream is \<surd> is the nth element of tsum5_h with the rest stream*)
+lemma tsum5_suc_snth_tick:"Fin n < #s \<and> shd s =\<surd> \<Longrightarrow> snth (Suc n) (tsum5_h m\<cdot>s) = snth n (tsum5_h m\<cdot>(srt\<cdot>s))"
+apply(subst tsum5_h_scons_tick_2)
 apply auto
 by (metis Fin_0 less_le lnle_Fin_0 strict_slen surj_scons)
 
-(**the (Suc nth) element of tsum5_helper m s when the head of the stream is not \<surd> is the nth element of tsum5_helper (m + shd s)  with the rest stream**)
-lemma tsum5_suc_snth:"Fin n < #s \<and> shd s \<noteq>\<surd> \<and> s\<noteq>\<epsilon> \<Longrightarrow> snth (Suc n) (tsum5_helper m\<cdot>s) = snth n (tsum5_helper (m+ \<M>\<inverse> shd s)\<cdot>(srt\<cdot>s))"
-apply(subst tsum5_helper_scons_2)
+(**the (Suc nth) element of tsum5_h m s when the head of the stream is not \<surd> is the nth element of tsum5_h (m + shd s)  with the rest stream**)
+lemma tsum5_suc_snth:"Fin n < #s \<and> shd s \<noteq>\<surd> \<and> s\<noteq>\<epsilon> \<Longrightarrow> snth (Suc n) (tsum5_h m\<cdot>s) = snth n (tsum5_h (m+ \<M>\<inverse> shd s)\<cdot>(srt\<cdot>s))"
+apply(subst tsum5_h_scons_2)
 by auto
 
-(*taking only \<surd>s of tsum5_helper is the same as taking \<surd>s of the input*)
-lemma tsum5_ticknum_helper[simp]: "({\<surd>} \<ominus> tsum5_helper n\<cdot>ts) =({\<surd>} \<ominus> ts) "
+(*taking only \<surd>s of tsum5_h is the same as taking \<surd>s of the input*)
+lemma tsum5_ticknum_helper[simp]: "({\<surd>} \<ominus> tsum5_h n\<cdot>ts) =({\<surd>} \<ominus> ts) "
 apply(cases "ts=\<epsilon>", simp)
 apply(induction ts arbitrary: n,auto)
 proof -
   fix u :: "nat event discr\<^sub>\<bottom>" and ts :: "nat event stream" and n:: nat
   assume a1: "u\<noteq>\<bottom>"
-  assume a2: "(\<And>n. ts \<noteq> \<epsilon> \<Longrightarrow> {\<surd>} \<ominus> tsum5_helper n\<cdot>ts = {\<surd>} \<ominus> ts)"
-  then show "{\<surd>} \<ominus> tsum5_helper n\<cdot>(u && ts) = {\<surd>} \<ominus> u && ts"
+  assume a2: "(\<And>n. ts \<noteq> \<epsilon> \<Longrightarrow> {\<surd>} \<ominus> tsum5_h n\<cdot>ts = {\<surd>} \<ominus> ts)"
+  then show "{\<surd>} \<ominus> tsum5_h n\<cdot>(u && ts) = {\<surd>} \<ominus> u && ts"
   apply(insert a1 a2)
   apply(cases "u=updis \<surd>")
   apply(insert lscons_conv[of \<surd> ts])
-  apply(subst tsum5_helper_scons_tick_2, auto)
+  apply(subst tsum5_h_scons_tick_2, auto)
   using a2 apply force
-  apply(subst tsum5_helper_scons_2)
+  apply(subst tsum5_h_scons_2)
   apply (metis stream.con_rews(2) stream.injects stream.sel_rews(5) surj_scons)
   apply simp
   using a2
@@ -304,56 +304,56 @@ proof -
 qed
 
 (*There are as much \<surd>s in the output as there are in the Input*)
-lemma tsum5_ticknum[simp]:"#({\<surd>} \<ominus> tsum5_helper 0\<cdot>ts) =#({\<surd>} \<ominus> ts)"
+lemma tsum5_ticknum[simp]:"#({\<surd>} \<ominus> tsum5_h 0\<cdot>ts) =#({\<surd>} \<ominus> ts)"
 by simp
 
 (*helper for tswell_tsum5*)
-lemma tsum5_srt2input:"(\<exists>x. srt\<cdot>(tsum5_helper n\<cdot>s) = tsum5_helper x\<cdot>(srt\<cdot>s))"
+lemma tsum5_srt2input:"(\<exists>x. srt\<cdot>(tsum5_h n\<cdot>s) = tsum5_h x\<cdot>(srt\<cdot>s))"
 apply(cases "s=\<epsilon>", simp)
 apply(cases "shd s=\<surd>")
-apply(subst tsum5_helper_scons_tick_2, auto)
+apply(subst tsum5_h_scons_tick_2, auto)
 using surj_scons apply fastforce
-by(subst tsum5_helper_scons_2, auto)
+by(subst tsum5_h_scons_2, auto)
 
 (*helper for tswell_tsum5*)
-lemma tsum5_sucn_sdrop:"(\<exists>x. sdrop (Suc n)\<cdot>(tsum5_helper 0\<cdot>s) = sdrop n\<cdot> (tsum5_helper x\<cdot>(srt\<cdot>s)))"
+lemma tsum5_sucn_sdrop:"(\<exists>x. sdrop (Suc n)\<cdot>(tsum5_h 0\<cdot>s) = sdrop n\<cdot> (tsum5_h x\<cdot>(srt\<cdot>s)))"
 apply(subst sdrop_forw_rt)
 using tsum5_srt2input
 by metis
 
 (*helper for tswell_tsum5*)
-lemma tsum5_sdrop2input:"(\<exists>x. sdrop n\<cdot>(tsum5_helper 0\<cdot>s) = tsum5_helper x\<cdot>(sdrop n\<cdot>s))"
+lemma tsum5_sdrop2input:"(\<exists>x. sdrop n\<cdot>(tsum5_h 0\<cdot>s) = tsum5_h x\<cdot>(sdrop n\<cdot>s))"
 apply(induction n arbitrary: s, auto)
 using tsum5_sucn_sdrop
-by (smt iterate_Suc lscons_conv sdrop_def stream.sel_rews(2) stream.sel_rews(5) surj_scons tsum5_empty tsum5_helper_scons tsum5_helper_srt_tick up_defined)
+by (smt iterate_Suc lscons_conv sdrop_def stream.sel_rews(2) stream.sel_rews(5) surj_scons tsum5_empty tsum5_h_scons tsum5_h_srt_tick up_defined)
 
 (*helper for tswell_tsum5*)
-lemma tsum5_snth2input:" (\<exists>x. snth n (tsum5_helper 0\<cdot>s) = shd (tsum5_helper x\<cdot> (sdrop n\<cdot> s)))"
+lemma tsum5_snth2input:" (\<exists>x. snth n (tsum5_h 0\<cdot>s) = shd (tsum5_h x\<cdot> (sdrop n\<cdot> s)))"
 apply(simp add: snth_def)
 using tsum5_sdrop2input by metis
 
 (*if the nth element of the input is a \<surd> so is the nth element of the output*)
-lemma tsum5_snthtick2output:" snth n s=\<surd> \<Longrightarrow> snth n (tsum5_helper 0\<cdot>s) =\<surd>"
+lemma tsum5_snthtick2output:" snth n s=\<surd> \<Longrightarrow> snth n (tsum5_h 0\<cdot>s) =\<surd>"
 apply(simp add: snth_def)
 apply(insert tsum5_snth2input[of n s])
 apply auto
-by (metis shd1 snth_def surj_scons tsum5_empty tsum5_helper_scons_tick)
+by (metis shd1 snth_def surj_scons tsum5_empty tsum5_h_scons_tick)
 
 (*if the input has a \<surd> at the end so does the output*)
-lemma tsum5_sfoot_helper:"#s<\<infinity> \<Longrightarrow> sfoot (tsum5_helper 0\<cdot>(s \<bullet> \<up>\<surd>)) = \<surd>"
+lemma tsum5_sfoot_helper:"#s<\<infinity> \<Longrightarrow> sfoot (tsum5_h 0\<cdot>(s \<bullet> \<up>\<surd>)) = \<surd>"
 apply(simp add: sfoot_def)
 apply(subst tsum5_snthtick2output, auto)
 by(insert sfoot12[of s \<surd>],simp add: sfoot_def)
 
-(*if the input of tsum5_helper is well formed so is the output*)
-lemma tswell_tsum5:"ts_well ts \<Longrightarrow> ts_well (tsum5_helper 0\<cdot>ts)"
+(*if the input of tsum5_h is well formed so is the output*)
+lemma tswell_tsum5:"ts_well ts \<Longrightarrow> ts_well (tsum5_h 0\<cdot>ts)"
 apply(cases "#ts=\<infinity>")
 apply(simp add: ts_well_def, auto)+
 using tsum5_sfoot_helper
 by (metis inf_ub less_le sconc_fst_inf sfoot2)
 
 (*unfolding of tsum5 with the definition*)
-lemma tsum5_unfold: "tsum5\<cdot> ts = Abs_tstream (tsum5_helper 0\<cdot> (Rep_tstream ts))"
+lemma tsum5_unfold: "tsum5\<cdot> ts = Abs_tstream (tsum5_h 0\<cdot> (Rep_tstream ts))"
 by (simp add: tsum5_def tswell_tsum5)
 
 
@@ -363,18 +363,18 @@ by (simp add: tsum5_def tswell_tsum5)
 lemma tswell_test: "ts_well ((<[n1,\<surd>,n2,\<surd>,\<surd>,n3]>) \<bullet> (sinftimes(\<up>\<surd>)))"
 by(simp add: ts_well_def)
 
-(*Result of the first part of the teststream with tsum5_helper 0*)
-lemma tsum5_helper_test_helper1: "tsum5_helper 0\<cdot>(<[\<M> 1,\<surd>,\<M> 2,\<surd>,\<surd>,\<M> 4]>) =(<[\<M> 1,\<surd>,\<M> 3,\<surd>,\<surd>,\<M> 7]>)"
-by (simp add: tsum5_helper_scons tsum5_helper_scons_tick)
+(*Result of the first part of the teststream with tsum5_h 0*)
+lemma tsum5_h_test_helper1: "tsum5_h 0\<cdot>(<[\<M> 1,\<surd>,\<M> 2,\<surd>,\<surd>,\<M> 4]>) =(<[\<M> 1,\<surd>,\<M> 3,\<surd>,\<surd>,\<M> 7]>)"
+by (simp add: tsum5_h_scons tsum5_h_scons_tick)
 
-(*result of the last part of the teststream with tsum5_helper n*)
-lemma tsum5_helper_test_helper2: "tsum5_helper n \<cdot>(sinftimes(\<up>\<surd>)) = sinftimes(\<up>\<surd>)"
-by (metis s2sinftimes sinftimes_unfold tsum5_helper_scons_tick)
+(*result of the last part of the teststream with tsum5_h n*)
+lemma tsum5_h_test_helper2: "tsum5_h n \<cdot>(sinftimes(\<up>\<surd>)) = sinftimes(\<up>\<surd>)"
+by (metis s2sinftimes sinftimes_unfold tsum5_h_scons_tick)
 
-(*result of the teststream with tsum5_helper 0*)
-lemma tsum5_helper_test: "tsum5_helper 0 \<cdot>((<[\<M> 1,\<surd>,\<M> 2,\<surd>,\<surd>,\<M> 4]>) \<bullet> (sinftimes(\<up>\<surd>))) = ((<[\<M> 1,\<surd>,\<M> 3,\<surd>,\<surd>,\<M> 7]>) \<bullet> (sinftimes(\<up>\<surd>)))"
-using tsum5_helper_test_helper1 tsum5_helper_test_helper2
-by (simp add: tsum5_helper_scons tsum5_helper_scons_tick)
+(*result of the teststream with tsum5_h 0*)
+lemma tsum5_h_test: "tsum5_h 0 \<cdot>((<[\<M> 1,\<surd>,\<M> 2,\<surd>,\<surd>,\<M> 4]>) \<bullet> (sinftimes(\<up>\<surd>))) = ((<[\<M> 1,\<surd>,\<M> 3,\<surd>,\<surd>,\<M> 7]>) \<bullet> (sinftimes(\<up>\<surd>)))"
+using tsum5_h_test_helper1 tsum5_h_test_helper2
+by (simp add: tsum5_h_scons tsum5_h_scons_tick)
 
 (*Tests the output of tsum5*)
 lemma tssum5_test:"tsum5\<cdot> (Abs_tstream ((<[\<M> 1, \<surd>, \<M> 2, \<surd>, \<surd>, \<M> 4]>) \<bullet> (sinftimes(\<up>\<surd>))))
@@ -382,8 +382,8 @@ lemma tssum5_test:"tsum5\<cdot> (Abs_tstream ((<[\<M> 1, \<surd>, \<M> 2, \<surd
 apply(simp add: tsum5_unfold)
 apply (subst Rep_Abs)
 using tswell_test apply auto
-using tsum5_helper_test_helper2
-by (simp add: tsum5_helper_scons tsum5_helper_scons_tick)
+using tsum5_h_test_helper2
+by (simp add: tsum5_h_scons tsum5_h_scons_tick)
 
 
 (*tsAbs(tsum5 ts) = sum5(tsAbs ts)*)
@@ -392,9 +392,9 @@ by (simp add: tsum5_helper_scons tsum5_helper_scons_tick)
 lemma[simp]:"\<M>\<inverse> (\<M> a) = a "
 by simp
 
-(*the (Suc nth) element of tsum5_helper m s of a stream without \<surd>s is the nth element of tsum5_helper (m+ shd s) with the rest stream*)
-lemma tsum5_sfilter_snth_helper:"Fin n < #({e. e\<noteq>\<surd>}\<ominus> s) \<and> ({e. e\<noteq>\<surd>}\<ominus> s)\<noteq>\<epsilon> \<Longrightarrow> snth (Suc n) (tsum5_helper m\<cdot>({e. e\<noteq>\<surd>}\<ominus> s)) = snth n (tsum5_helper (m+ \<M>\<inverse> shd ({e. e\<noteq>\<surd>}\<ominus> s))\<cdot>(srt\<cdot>({e. e\<noteq>\<surd>}\<ominus> s)))"
-apply(subst tsum5_helper_scons_2)
+(*the (Suc nth) element of tsum5_h m s of a stream without \<surd>s is the nth element of tsum5_h (m+ shd s) with the rest stream*)
+lemma tsum5_sfilter_snth_helper:"Fin n < #({e. e\<noteq>\<surd>}\<ominus> s) \<and> ({e. e\<noteq>\<surd>}\<ominus> s)\<noteq>\<epsilon> \<Longrightarrow> snth (Suc n) (tsum5_h m\<cdot>({e. e\<noteq>\<surd>}\<ominus> s)) = snth n (tsum5_h (m+ \<M>\<inverse> shd ({e. e\<noteq>\<surd>}\<ominus> s))\<cdot>(srt\<cdot>({e. e\<noteq>\<surd>}\<ominus> s)))"
+apply(subst tsum5_h_scons_2)
 using sfilter_ne_resup apply auto[1]
 by auto
 
@@ -405,27 +405,27 @@ using ex_snth_in_sfilter_nempty by auto
 lemma sfilter_length_srt: "#({a}\<ominus> (srt\<cdot>s)) \<le> #({a}\<ominus> s)"
 by (metis (no_types, lifting) eq_iff less_lnsuc sfilter_in sfilter_nin slen_scons stream.sel_rews(2) surj_scons)
 
-(*helper for tsum5_helper_sfilter_snth*)
+(*helper for tsum5_h_sfilter_snth*)
 lemma sfilter_filtered_len_srt: "({a} \<ominus> (srt\<cdot>({e. e \<noteq> a} \<ominus> s))) = \<epsilon>"
 by (metis (mono_tags, lifting) mem_Collect_eq sdom_sfilter1 sfilter2dom sfilter_srtdwl3)
 
-(*The nat of snth nat event of tsum5_helper m s is the snth of tsum5_helper 0 s + m*)
-lemma tsum5_sfilter_snth_unfold:"Fin n < #s \<and> #({\<surd>}\<ominus> s) = 0 \<Longrightarrow> \<M>\<inverse> snth n (tsum5_helper m\<cdot>s) = \<M>\<inverse> snth n (tsum5_helper 0\<cdot>s) + m"
+(*The nat of snth nat event of tsum5_h m s is the snth of tsum5_h 0 s + m*)
+lemma tsum5_sfilter_snth_unfold:"Fin n < #s \<and> #({\<surd>}\<ominus> s) = 0 \<Longrightarrow> \<M>\<inverse> snth n (tsum5_h m\<cdot>s) = \<M>\<inverse> snth n (tsum5_h 0\<cdot>s) + m"
 apply(induction n arbitrary: m s, simp)
-apply(subst tsum5_helper_scons_2)
+apply(subst tsum5_h_scons_2)
 apply (metis lnsuc_neq_0_rev sfilter_in singletonI slen_empty_eq slen_scons surj_scons)
-apply (subst tsum5_helper_shd_2)
+apply (subst tsum5_h_shd_2)
 apply (metis lnsuc_neq_0_rev sfilter_in singletonI slen_empty_eq slen_scons surj_scons)
 apply simp
 apply simp
 apply(simp add: snth_rt)
-apply(insert tsum5_helper_srt, auto)
+apply(insert tsum5_h_srt, auto)
 by (smt Fin_Suc add.commute add.left_commute insert_iff less_imp_not_less lnle_Fin_0 lnsuc_lnle_emb lscons_conv not_less old.nat.distinct(2) ord_eq_less_trans sfilter_in sfilter_nin slen_empty_eq slen_scons stream.con_rews(2) surj_scons)
 
 
-(*without \<surd>s in stream tsum5_helper unfolding the snth+1 element *)
-lemma tsum5_helper_sfilter_snth:"Fin (Suc n) < #({e. e\<noteq>\<surd>}\<ominus> s) \<and> ({e. e\<noteq>\<surd>}\<ominus> s)\<noteq>\<epsilon> \<Longrightarrow> 
-\<M>\<inverse> snth (Suc n) (tsum5_helper m\<cdot>({e. e\<noteq>\<surd>}\<ominus> s)) = \<M>\<inverse> snth n (tsum5_helper 0\<cdot>(srt\<cdot>({e. e\<noteq>\<surd>}\<ominus> s))) +(m+ \<M>\<inverse> shd ({e. e\<noteq>\<surd>}\<ominus> s))"
+(*without \<surd>s in stream tsum5_h unfolding the snth+1 element *)
+lemma tsum5_h_sfilter_snth:"Fin (Suc n) < #({e. e\<noteq>\<surd>}\<ominus> s) \<and> ({e. e\<noteq>\<surd>}\<ominus> s)\<noteq>\<epsilon> \<Longrightarrow> 
+\<M>\<inverse> snth (Suc n) (tsum5_h m\<cdot>({e. e\<noteq>\<surd>}\<ominus> s)) = \<M>\<inverse> snth n (tsum5_h 0\<cdot>(srt\<cdot>({e. e\<noteq>\<surd>}\<ominus> s))) +(m+ \<M>\<inverse> shd ({e. e\<noteq>\<surd>}\<ominus> s))"
 apply(subst tsum5_sfilter_snth_helper)
 apply simp
 apply (metis Fin_leq_Suc_leq Suc_n_not_le_n less2nat_lemma less_le)
@@ -435,8 +435,8 @@ apply (metis Fin_Suc lnsuc_lnle_emb not_less slen_scons surj_scons)
 by simp
 
 lemma tsum5_sfilter_snth:"Fin (Suc n) < #({e. e\<noteq>\<surd>}\<ominus> s) \<and> ({e. e\<noteq>\<surd>}\<ominus> s)\<noteq>\<epsilon> \<Longrightarrow> 
-\<M>\<inverse> snth (Suc n) (tsum5_helper 0\<cdot>({e. e\<noteq>\<surd>}\<ominus> s)) = \<M>\<inverse> snth n (tsum5_helper 0\<cdot>(srt\<cdot>({e. e\<noteq>\<surd>}\<ominus> s))) +\<M>\<inverse> shd ({e. e\<noteq>\<surd>}\<ominus> s)"
-by(insert tsum5_helper_sfilter_snth [of n s 0], simp)
+\<M>\<inverse> snth (Suc n) (tsum5_h 0\<cdot>({e. e\<noteq>\<surd>}\<ominus> s)) = \<M>\<inverse> snth n (tsum5_h 0\<cdot>(srt\<cdot>({e. e\<noteq>\<surd>}\<ominus> s))) +\<M>\<inverse> shd ({e. e\<noteq>\<surd>}\<ominus> s)"
+by(insert tsum5_h_sfilter_snth [of n s 0], simp)
 
 lemma sum3_snth_2:"Fin (Suc n) < #s \<Longrightarrow> snth (Suc n) (sum3\<cdot>s) = snth n (sum3\<cdot>(srt\<cdot>s)) + shd s"
 apply(insert sum3_snth[of n s 0], simp)
@@ -455,10 +455,10 @@ by (metis less_le lnle_Fin_0 nat.distinct(1) not_less slen_rt_ile_eq strict_slen
 lemma sfilter_sfilter[simp]: "{a}\<ominus>{a}\<ominus>s = {a}\<ominus>s"
 by simp
 
-lemma tsum5_helper_snth2sum3_snth:"Fin n < #({e. e\<noteq>\<surd>}\<ominus> s) \<and> ({e. e\<noteq>\<surd>}\<ominus> s)\<noteq>\<epsilon> \<Longrightarrow>
- \<M>\<inverse> snth n (tsum5_helper 0\<cdot>({e. e\<noteq>\<surd>}\<ominus> s)) = snth n (sum3\<cdot>(smap (\<lambda>e. \<M>\<inverse> e)\<cdot>({e. e\<noteq>\<surd>}\<ominus> s)))"
+lemma tsum5_h_snth2sum3_snth:"Fin n < #({e. e\<noteq>\<surd>}\<ominus> s) \<and> ({e. e\<noteq>\<surd>}\<ominus> s)\<noteq>\<epsilon> \<Longrightarrow>
+ \<M>\<inverse> snth n (tsum5_h 0\<cdot>({e. e\<noteq>\<surd>}\<ominus> s)) = snth n (sum3\<cdot>(smap (\<lambda>e. \<M>\<inverse> e)\<cdot>({e. e\<noteq>\<surd>}\<ominus> s)))"
 apply(induction n arbitrary: s, simp+)
-apply(subst tsum5_helper_shd_2, simp)
+apply(subst tsum5_h_shd_2, simp)
 using sfilter_ne_resup apply auto[1]
 apply simp
 apply(subst tsum5_sfilter_snth)
@@ -469,50 +469,50 @@ apply simp
 by (smt inject_scons less2lnleD lnle_Fin_0 nat.distinct(1) not_less sfilter_srtdwl3 slen_rt_ile_eq slen_smap smap1 smap_split strict_slen surj_scons)
 
 (*helper for tsum52sum4_helper*)
-lemma tsum5_helper2sum3:"smap (\<lambda>e. \<M>\<inverse> e)\<cdot> (tsum5_helper 0\<cdot>({e. e\<noteq>\<surd>}\<ominus> s)) = sum3\<cdot>(smap (\<lambda>e. \<M>\<inverse> e)\<cdot>({e. e\<noteq>\<surd>}\<ominus> s))"
+lemma tsum5_h2sum3:"smap (\<lambda>e. \<M>\<inverse> e)\<cdot> (tsum5_h 0\<cdot>({e. e\<noteq>\<surd>}\<ominus> s)) = sum3\<cdot>(smap (\<lambda>e. \<M>\<inverse> e)\<cdot>({e. e\<noteq>\<surd>}\<ominus> s))"
 apply(rule snths_eq, simp)
 apply auto
 apply(subst smap_snth_lemma)
 apply simp
-apply(rule tsum5_helper_snth2sum3_snth, auto)
+apply(rule tsum5_h_snth2sum3_snth, auto)
 by (metis Fin_0 less_le lnle_Fin_0)
 
 (*If you filter out \<surd>s the length of the input stream is equal to the length of the output stream*)
-lemma sfilter_in_tsum_helper_len[simp]: " #({e. e \<noteq> \<surd>} \<ominus> tsum5_helper n\<cdot>ts) = #({e. e \<noteq> \<surd>} \<ominus> ts)"
+lemma sfilter_in_tsum_helper_len[simp]: " #({e. e \<noteq> \<surd>} \<ominus> tsum5_h n\<cdot>ts) = #({e. e \<noteq> \<surd>} \<ominus> ts)"
 apply(induction ts arbitrary: n, auto)
 proof -
   fix u :: "nat event discr\<^sub>\<bottom>" and ts :: "nat event stream" and n:: nat
   assume a1: "u\<noteq>\<bottom>"
-  assume a2: "(\<And>n. #({e. e \<noteq> \<surd>} \<ominus> tsum5_helper n\<cdot>ts) = #({e. e \<noteq> \<surd>} \<ominus> ts))"
-  then show "#({e. e \<noteq> \<surd>} \<ominus> tsum5_helper n\<cdot>(u && ts)) = #({e. e \<noteq> \<surd>} \<ominus> u && ts)"
+  assume a2: "(\<And>n. #({e. e \<noteq> \<surd>} \<ominus> tsum5_h n\<cdot>ts) = #({e. e \<noteq> \<surd>} \<ominus> ts))"
+  then show "#({e. e \<noteq> \<surd>} \<ominus> tsum5_h n\<cdot>(u && ts)) = #({e. e \<noteq> \<surd>} \<ominus> u && ts)"
   apply(insert a1 a2)
   apply(cases "u=updis \<surd>")
   apply(insert lscons_conv[of \<surd> ts])
-  apply(subst tsum5_helper_scons_tick_2, auto)
-  apply(subst tsum5_helper_scons_2)
+  apply(subst tsum5_h_scons_tick_2, auto)
+  apply(subst tsum5_h_scons_2)
   apply (metis stream.con_rews(2) stream.injects stream.sel_rews(5) surj_scons)
   apply simp
 by (smt lshd_updis mem_Collect_eq sfilter_in slen_scons stream.con_rews(2) stream.sel_rews(4) stream.sel_rews(5) surj_scons)
 qed
 
 (*it does not matter if i filter out the \<surd>s in at the input or the output*)
-lemma sfilter_in_tsum5:"{e. e \<noteq> \<surd>} \<ominus> tsum5_helper n\<cdot>ts = tsum5_helper n\<cdot>({e. e \<noteq> \<surd>} \<ominus> ts)"
+lemma sfilter_in_tsum5:"{e. e \<noteq> \<surd>} \<ominus> tsum5_h n\<cdot>ts = tsum5_h n\<cdot>({e. e \<noteq> \<surd>} \<ominus> ts)"
 apply(cases "ts=\<epsilon>",simp)
 apply(induction ts arbitrary: n, auto)
 proof -
   fix u :: "nat event discr\<^sub>\<bottom>" and ts :: "nat event stream" and n:: nat
   assume a1: "u\<noteq>\<bottom>"
-  assume a2: "(\<And>n. ts \<noteq> \<epsilon> \<Longrightarrow> {e. e \<noteq> \<surd>} \<ominus> tsum5_helper n\<cdot>ts = tsum5_helper n\<cdot>({e. e \<noteq> \<surd>} \<ominus> ts))"
-  then show "{e. e \<noteq> \<surd>} \<ominus> tsum5_helper n\<cdot>(u && ts) = tsum5_helper n\<cdot>({e. e \<noteq> \<surd>} \<ominus> u && ts)"
+  assume a2: "(\<And>n. ts \<noteq> \<epsilon> \<Longrightarrow> {e. e \<noteq> \<surd>} \<ominus> tsum5_h n\<cdot>ts = tsum5_h n\<cdot>({e. e \<noteq> \<surd>} \<ominus> ts))"
+  then show "{e. e \<noteq> \<surd>} \<ominus> tsum5_h n\<cdot>(u && ts) = tsum5_h n\<cdot>({e. e \<noteq> \<surd>} \<ominus> u && ts)"
   apply(insert a1 a2)
   apply(cases "u=updis \<surd>")
   apply(insert lscons_conv[of \<surd> ts])
-  apply(subst tsum5_helper_scons_tick_2, auto)
+  apply(subst tsum5_h_scons_tick_2, auto)
   apply fastforce
-  apply(subst tsum5_helper_scons_2)
+  apply(subst tsum5_h_scons_2)
   apply (metis stream.con_rews(2) stream.injects stream.sel_rews(5) surj_scons)
   apply simp
-  by (smt mem_Collect_eq sfilter_in stream.con_rews(2) stream.injects stream.sel_rews(5) strict_sfilter surj_scons tsum5_empty tsum5_helper_scons)
+  by (smt mem_Collect_eq sfilter_in stream.con_rews(2) stream.injects stream.sel_rews(5) strict_sfilter surj_scons tsum5_empty tsum5_h_scons)
 qed
 
 (*helper for tsum52sum4*)
@@ -521,7 +521,7 @@ apply(subst tsum5_unfold)
 apply(subst Rep_Abs)
 using tswell_tsum5 apply auto
 apply(subst sfilter_in_tsum5)
-apply(subst tsum5_helper2sum3)
+apply(subst tsum5_h2sum3)
 by simp
 
 (*tsum5 and sum4 work the same way over naturals*)
@@ -530,12 +530,14 @@ apply(simp add: tsabs_insert)
 by(rule tsum52sum3_helper)
 
 (*shows that tsum5 is a weak causal*)
-lemma"tsWeakCausal (\<lambda> ts. Abs_tstream (tsum5_helper 0\<cdot>(Rep_tstream ts)))"
+lemma tsWeak2tsum5:"tsWeakCausal (\<lambda> ts. Abs_tstream (tsum5_h 0\<cdot>(Rep_tstream ts)))"
 apply(subst tsWeak2cont2)
 apply(simp add: tsTickCount_def)
 apply(subst Rep_Abs, auto)
 by(simp add: tswell_tsum5)+
 
+lemma tsWeak_tsum5:"tsWeakCausal(\<lambda> ts. tsum5\<cdot>ts)"
+by(simp add: tsum5_unfold tsWeak2tsum5)
 
 (*definition tsum_nth like sum_nth*)
 primrec tsum_nth:: "nat \<Rightarrow> nat event stream \<Rightarrow> nat" where
@@ -545,8 +547,8 @@ primrec tsum_nth:: "nat \<Rightarrow> nat event stream \<Rightarrow> nat" where
 
 
 (*if the nth element of the output is a \<surd> so is the nth element of the input*)
-lemma tsum5_snthtick2input:" snth n (tsum5_helper 0\<cdot>s) =\<surd> \<Longrightarrow> snth n s =\<surd>"
-by (metis event.distinct(1) shd1 snth_def surj_scons tsum5_empty tsum5_helper_scons tsum5_sdrop2input)
+lemma tsum5_snthtick2input:" snth n (tsum5_h 0\<cdot>s) =\<surd> \<Longrightarrow> snth n s =\<surd>"
+by (metis event.distinct(1) shd1 snth_def surj_scons tsum5_empty tsum5_h_scons tsum5_sdrop2input)
 
 (*if the shd s is \<surd> the sum of s is the sum of the rest of s*)
 lemma tsum_nth_suc_tick: "shd s=\<surd> \<Longrightarrow> tsum_nth (Suc n) s = tsum_nth n (srt\<cdot>s)"
@@ -556,51 +558,51 @@ by(simp add: tsum_nth_def)
 lemma tsum_nth_suc: "shd s\<noteq>\<surd> \<Longrightarrow> tsum_nth (Suc n) s = \<M>\<inverse> shd s + tsum_nth n (srt\<cdot>s)"
 by(simp add: tsum_nth_def)
 
-(*simps \<M> and \<M>\<inverse>*)
-lemma[simp]: "x\<noteq>\<surd> \<Longrightarrow> \<M> \<M>\<inverse>x=x"
+(* \<M> before \<M>\<inverse>*)
+lemma MsginvMsg: "x\<noteq>\<surd> \<Longrightarrow> \<M> \<M>\<inverse>x=x"
 by (metis event.exhaust event.simps(4))
 
-(*helper for tsum5_helper_2tsum_tnh_helper*)
-lemma tsum5_helper_extract_state:"Fin n < #s \<and>  snth n s \<noteq> \<surd> \<and> s\<noteq>\<epsilon> \<Longrightarrow> snth n (tsum5_helper m\<cdot>s) = \<M> \<M>\<inverse> snth n (tsum5_helper 0\<cdot>s) + m"
+(*helper for tsum5_h_2tsum_tnh_helper*)
+lemma tsum5_h_extract_state:"Fin n < #s \<and>  snth n s \<noteq> \<surd> \<and> s\<noteq>\<epsilon> \<Longrightarrow> snth n (tsum5_h m\<cdot>s) = \<M> \<M>\<inverse> snth n (tsum5_h 0\<cdot>s) + m"
 apply(induction n arbitrary: m s, auto)
 apply(simp add: snth_rt)
 proof -
   fix s :: "nat event stream" and n:: nat and m:: nat
-  assume a1: "(\<And>m s. Fin n < #s \<and> snth n s \<noteq> \<surd> \<and> s \<noteq> \<epsilon> \<Longrightarrow> snth n (tsum5_helper m\<cdot>s) = \<M> \<M>\<inverse> snth n (tsum5_helper 0\<cdot>s) + m)"
+  assume a1: "(\<And>m s. Fin n < #s \<and> snth n s \<noteq> \<surd> \<and> s \<noteq> \<epsilon> \<Longrightarrow> snth n (tsum5_h m\<cdot>s) = \<M> \<M>\<inverse> snth n (tsum5_h 0\<cdot>s) + m)"
   assume a2: "Fin (Suc n) < #s"
   assume a3: " snth n (srt\<cdot>s) \<noteq> \<surd>"
   assume a4: "s \<noteq> \<epsilon>"
-  then show "snth n (srt\<cdot>(tsum5_helper m\<cdot>s)) = \<M> \<M>\<inverse> snth n (srt\<cdot>(tsum5_helper 0\<cdot>s)) + m"
+  then show "snth n (srt\<cdot>(tsum5_h m\<cdot>s)) = \<M> \<M>\<inverse> snth n (srt\<cdot>(tsum5_h 0\<cdot>s)) + m"
   apply(cases "shd s=\<surd>")
-  apply(simp add: tsum5_helper_srt_tick)
+  apply(simp add: tsum5_h_srt_tick)
   apply(insert a1 a2 a3)
   apply(metis less2lnleD lnle_Fin_0 nat.distinct(1) not_less slen_rt_ile_eq strict_slen)
-  apply(simp add: tsum5_helper_srt)
+  apply(simp add: tsum5_h_srt)
   by (smt a2 add.left_commute add.right_neutral event.inject event.simps(4) less2lnleD lnle_Fin_0 not_le old.nat.distinct(2) slen_empty_eq slen_rt_ile_eq)
 qed
 
 
 (*if the nth element of the input is not \<surd>, then the nth element of the output is equal to tsum_nth n input*)
-lemma tsum5_helper2tsum_nth_helper:"Fin n < #s \<Longrightarrow> snth n s \<noteq> \<surd> \<Longrightarrow> snth n (tsum5_helper 0\<cdot>s) = \<M> tsum_nth n s"
+lemma tsum5_h2tsum_nth_helper:"Fin n < #s \<Longrightarrow> snth n s \<noteq> \<surd> \<Longrightarrow> snth n (tsum5_h 0\<cdot>s) = \<M> tsum_nth n s"
 apply(cases "s=\<epsilon>")
-apply(simp add: lnless_def)
+apply(simp add: lnless_def MsginvMsg)
 apply(induction n arbitrary: s,auto)
 apply(subst tsum5_suc_snth_tick)
 apply(metis Fin_leq_Suc_leq less_le not_le)
 apply (metis less2lnleD lnle_Fin_0 nat.distinct(1) not_le slen_rt_ile_eq snth_rt strict_slen)
-apply(subst tsum5_helper_scons_2,simp+)
-apply(subst tsum5_helper_extract_state)
+apply(subst tsum5_h_scons_2,simp+)
+apply(subst tsum5_h_extract_state)
 apply (metis less2lnleD lnle_Fin_0 nat.simps(3) not_le slen_rt_ile_eq snth_rt strict_slen)
 apply auto
 by (metis event.simps(4) less2lnleD lnle_Fin_0 not_le old.nat.distinct(2) slen_empty_eq slen_rt_ile_eq snth_rt)
 
 
 (*helper for tsum52tsum_nth*)
-lemma tsum5_helper2tsum_nth:"Fin n< #s \<Longrightarrow> snth n (tsum5_helper 0\<cdot> s) = (case (snth n s) of Msg a \<Rightarrow> \<M> tsum_nth n s | \<surd> \<Rightarrow> \<surd>)"
+lemma tsum5_h2tsum_nth:"Fin n< #s \<Longrightarrow> snth n (tsum5_h 0\<cdot> s) = (case (snth n s) of Msg a \<Rightarrow> \<M> tsum_nth n s | \<surd> \<Rightarrow> \<surd>)"
 apply(cases "snth n s =\<surd>")
 apply(induction n arbitrary: s, simp add: tsum5_shd)
 apply(subst tsum5_snthtick2output, auto)
-apply(subst tsum5_helper2tsum_nth_helper, auto)
+apply(subst tsum5_h2tsum_nth_helper, auto)
 by (metis event.exhaust event.simps(4))
 
 (*if the nth element of the input is \<surd>, so is the nth element of the output. Otherwise it is tsum n input for the nth element*)
@@ -608,9 +610,30 @@ lemma tsum52tsum_nth:"Fin n< #(Rep_tstream ts) \<Longrightarrow> snth n (Rep_tst
 apply(simp add: tsum5_unfold)
 apply(subst Rep_Abs)
 using tswell_tsum5 apply simp
-by(subst tsum5_helper2tsum_nth, simp+)
+by(subst tsum5_h2tsum_nth, simp+)
+
+
+lemma tsum_nth_shd:"shd s\<noteq>\<surd> \<Longrightarrow> tsum_nth 0 s = \<M>\<inverse>shd s"
+by auto
+
+lemma "({e. e\<noteq>\<surd>}\<ominus> s) \<noteq>\<epsilon> \<Longrightarrow> shd ({e. e \<noteq> \<surd>} \<ominus> s) \<noteq> \<surd>"
+using sfilter_ne_resup by auto
+
+lemma filtereps2tsAbseps:"ts_well s \<and> {e. e \<noteq> \<surd>} \<ominus> s = \<epsilon> \<Longrightarrow> tsAbs\<cdot>(Abs_tstream s) = \<epsilon>"
+by(subst tsabs_insert, simp)
 
 (*
+lemma tsum_nth2sum_nth:"({e. e\<noteq>\<surd>}\<ominus> s) \<noteq> \<epsilon> \<Longrightarrow>ts_well s \<Longrightarrow> tsum_nth n ({e. e\<noteq>\<surd>}\<ominus> s) = sum_nth n (tsAbs\<cdot>(Abs_tstream s))"
+apply(induction n arbitrary: s)
+apply(subst tsum_nth_shd)
+using sfilter_ne_resup mem_Collect_eq apply blast
+apply(subst sum_nth.simps)
+apply(simp add: tsabs_rep_eq)
+apply(subst tsum_nth_suc)
+
+sorry
+
 lemma "snth n (Rep_tstream(tsum5\<cdot> ts)) = (case (snth n (Rep_tstream ts)) of Msg a \<Rightarrow> \<M> sum_stream (stake n\<cdot>(Rep_tstream ts)) | \<surd> \<Rightarrow> \<surd>)"
 *)
+
 end
